{
 "cells": [
  {
   "cell_type": "markdown",
   "id": "41940b8d",
   "metadata": {},
   "source": [
    "$\\textbf{Shion Suzuki BSCS-1}$\n",
    "\n",
    "$\\textbf{23101060}$"
   ]
  },
  {
   "cell_type": "markdown",
   "id": "188d623d-79cb-4d7e-aaed-112bb84d8d33",
   "metadata": {},
   "source": [
    "$\\textbf{Assignment}$\n",
    "Instructions:\n",
    "- Use latex.\n",
    "- Write your latex in jupyter notebook.\n",
    "- Push your answer to your github account.\n",
    "- Deadline is 2 weeks before finals.\n",
    "- Fail to submit 2 weeks before finals is an automatic 5.0 for this assignment.\n",
    "- Each problem is 25 points.\n",
    "\n",
    "1. Recall the definition of a rational number, denoted as $\\mathbb{Q}$. Prove that the Euler's number $e = \\Sigma_{k=0}^\\infty \\frac{1}{k!} \\notin \\mathbb{Q}$. A factorial is defined as $k! = (k)(k-1)(k-2)(k-3)..., \\forall k \\in \\mathbb{Z}^+$, note that $0! = 1$. Furthermore, a sum notation $\\Sigma_{k=0}^\\infty k = 0+ 1 + 2 + 3 +....+...$\n",
    "\n",
    "\n",
    "\n",
    "2. Prove Minkowski's Inequality for sums, $\\forall \\ p>1, (a_k, b_k)>0$:\n",
    "\n",
    "\\begin{gather}\n",
    "\\begin{bmatrix}\n",
    "\\Sigma_{k=1}^n |a_k + b_k|^p\n",
    "\\end{bmatrix}^\\frac{1}{p}\n",
    "\\leq\n",
    "\\begin{bmatrix}\n",
    "\\Sigma_{k=1}^n |a_k|^p\n",
    "\\end{bmatrix}^\\frac{1}{p}\n",
    "\n",
    "\\begin{bmatrix}\n",
    "\\Sigma_{k=1}^n |b_k|^p\n",
    "\\end{bmatrix}^\\frac{1}{p}\n",
    "\\end{gather}\n",
    "\n",
    "3. Prove the triangle inequality $|x+y| \\leq |x| + |y|, \\forall (x,y) \\in \\mathbb{R}$\n",
    "\n",
    "4. Prove Sedrakayan's Lemma $\\forall u_i, v_i \\in \\mathbb{R}^+$:\n",
    "\\begin{gather}\n",
    "\\frac{(\\Sigma_{i=1}^n u_i)^2}{\\Sigma_{i=1}^n v_i}\n",
    "\\leq\n",
    "\\Sigma_{i=1}^n \\frac{(u_i)^2}{v_i}\n",
    "\\end{gather}"
   ]
  },
  {
   "cell_type": "markdown",
   "id": "1de33a92-7a6a-4624-a8c5-994644cffc20",
   "metadata": {},
   "source": [
    "1. Consider the functions $f(x) = 2x+1$, $g(x)=2y-1$, $j(x) = |f(x)+g(x)|$, and $h(x) = j(x)^2$, show for the following inequality that:\n",
    "\n",
    "\\begin{gather}\n",
    "\\sqrt{|f(x)|^2} \\geq \\sqrt{h(x)} - \\sqrt{|g(x)|^2}, \\forall (x,y) \\in \\mathbb{Z}^+\n",
    "\\end{gather}"
   ]
  },
  {
   "cell_type": "markdown",
   "id": "997eb723-4112-443b-92d6-4f6734ea8e3b",
   "metadata": {},
   "source": [
    "2. Prove Sedrakayan's Lemma if $u_i, v_i$ are square roots of an even integers:\n",
    "\\begin{gather}\n",
    "\\frac{(\\Sigma_{i=1}^n u_i)^2}{\\Sigma_{i=1}^n v_i}\n",
    "\\leq\n",
    "\\Sigma_{i=1}^n \\frac{(u_i)^2}{v_i}\n",
    "\\end{gather}"
   ]
  },
  {
   "cell_type": "markdown",
   "id": "73beafe7",
   "metadata": {},
   "source": [
    "$\\textbf{Answers:}$\n",
    "-"
   ]
  },
  {
   "cell_type": "markdown",
   "id": "83da31f5",
   "metadata": {},
   "source": [
    "---\n",
    "### Question 1:\n",
    "Recall the definition of a rational number, denoted as $\\mathbb{Q}$. Prove that the Euler's number $e = \\Sigma_{k=0}^\\infty \\frac{1}{k!} \\notin \\mathbb{Q}$. A factorial is defined as $k! = (k)(k-1)(k-2)(k-3)..., \\forall k \\in \\mathbb{Z}^+$, note that $0! = 1$. Furthermore, a sum notation $\\Sigma_{k=0}^\\infty k = 0+ 1 + 2 + 3 +....+...$\n",
    "\n",
    "To prove that Euler's number $ e $ is not rational, we can use a proof by contradiction. Suppose $ e $ is rational, meaning it can be expressed as a fraction $ \\frac{p}{q} $ where $ p $ and $ q $ are integers with no common factors other than 1, and $ q \\neq 0 $.\n",
    "\n",
    "The Taylor series expansion of $ e $ is:\n",
    "\n",
    "$ e = \\sum_{k=0}^\\infty \\frac{1}{k!} = 1 + \\frac{1}{1!} + \\frac{1}{2!} + \\frac{1}{3!} + \\cdots $\n",
    "\n",
    "Now, let's denote the sum of the first $ n $ terms of the series as $ S_n $:\n",
    "\n",
    "$ S_n = 1 + \\frac{1}{1!} + \\frac{1}{2!} + \\frac{1}{3!} + \\cdots + \\frac{1}{n!} $\n",
    "\n",
    "We'll now multiply both sides of this equation by $ q! $, which is a positive integer for all $ q \\geq 0 $:\n",
    "\n",
    "$ q! \\cdot S_n = q! + q! \\frac{1}{1!} + q! \\frac{1}{2!} + q! \\frac{1}{3!} + \\cdots + q! \\frac{1}{n!} $\n",
    "\n",
    "This can be rewritten as:\n",
    "\n",
    "$ q! \\cdot S_n = q! + q! + \\frac{q!}{2!} + \\frac{q!}{3!} + \\cdots + \\frac{q!}{n!} $\n",
    "\n",
    "Notice that each term in the sum is an integer since it's a product of integers. Therefore, $ q! \\cdot S_n $ is an integer.\n",
    "\n",
    "Now, if $ e $ were rational, there would exist some integer $ N $ such that for all $ n \\geq N $, $ S_n = \\frac{p}{q} $, where $ p $ and $ q $ are integers with no common factors other than 1.\n",
    "\n",
    "But we've just shown that $ q! \\cdot S_n $ is always an integer. Therefore, for any choice of $ N $, there exists $ n \\geq N $ such that $ q! \\cdot S_n $ is not equal to $ p $, which contradicts the assumption that $ e $ is rational.\n",
    "\n",
    "Hence, Euler's number $ e $ is irrational.\n",
    "\n",
    "---\n",
    "\n",
    "### Question 2:\n",
    "Prove Minkowski's Inequality for sums, $\\forall \\ p>1, (a_k, b_k)>0$:\n",
    "\n",
    "To prove Minkowski's Inequality for sums, let's consider two sequences of real numbers $\\{a_k\\}$ and $\\{b_k\\}$, both indexed by $k$ from 1 to $n$, and a real number $p > 1$. Minkowski's Inequality states:\n",
    "\n",
    "$$\n",
    "\\left( \\sum_{k=1}^{n} (a_k + b_k)^p \\right)^{\\frac{1}{p}} \\leq \\left( \\sum_{k=1}^{n} a_k^p \\right)^{\\frac{1}{p}} + \\left( \\sum_{k=1}^{n} b_k^p \\right)^{\\frac{1}{p}}\n",
    "$$\n",
    "\n",
    "1. **Base Case**: Start with $n = 1$. The inequality trivially holds in this case since it reduces to the triangle inequality for real numbers.\n",
    "\n",
    "2. **Inductive Step**: Assume that Minkowski's Inequality holds for some positive integer $n = m$, i.e.,\n",
    "\n",
    "   $$\n",
    "   \\left( \\sum_{k=1}^{m} (a_k + b_k)^p \\right)^{\\frac{1}{p}} \\leq \\left( \\sum_{k=1}^{m} a_k^p \\right)^{\\frac{1}{p}} + \\left( \\sum_{k=1}^{m} b_k^p \\right)^{\\frac{1}{p}}\n",
    "   $$\n",
    "\n",
    "3. **Proving for $n = m + 1$**:\n",
    "\n",
    "   Consider the $n = m + 1$ case:\n",
    "\n",
    "   $$\n",
    "   \\left( \\sum_{k=1}^{m+1} (a_k + b_k)^p \\right)^{\\frac{1}{p}}\n",
    "   $$\n",
    "\n",
    "   Using the triangle inequality, we have:\n",
    "\n",
    "   $$\n",
    "   \\leq \\left( \\left( \\sum_{k=1}^{m} (a_k + b_k)^p \\right)^{\\frac{1}{p}} + (a_{m+1} + b_{m+1})^p \\right)^{\\frac{1}{p}}\n",
    "   $$\n",
    "\n",
    "   Now, using the induction hypothesis, we know:\n",
    "\n",
    "   $$\n",
    "   \\left( \\sum_{k=1}^{m} (a_k + b_k)^p \\right)^{\\frac{1}{p}} \\leq \\left( \\sum_{k=1}^{m} a_k^p \\right)^{\\frac{1}{p}} + \\left( \\sum_{k=1}^{m} b_k^p \\right)^{\\frac{1}{p}}\n",
    "   $$\n",
    "\n",
    "   Substituting this into the previous expression:\n",
    "\n",
    "   $$\n",
    "   \\leq \\left( \\left( \\left( \\sum_{k=1}^{m} a_k^p \\right)^{\\frac{1}{p}} + \\left( \\sum_{k=1}^{m} b_k^p \\right)^{\\frac{1}{p}} \\right) + (a_{m+1} + b_{m+1})^p \\right)^{\\frac{1}{p}}\n",
    "   $$\n",
    "\n",
    "   By the convexity of the $p$-th power function, we have:\n",
    "\n",
    "   $$\n",
    "   \\leq \\left( \\left( \\left( \\sum_{k=1}^{m} a_k^p \\right)^{\\frac{1}{p}} \\right) + \\left( \\left( \\sum_{k=1}^{m} b_k^p \\right)^{\\frac{1}{p}} + (a_{m+1} + b_{m+1})^p \\right) \\right)^{\\frac{1}{p}}\n",
    "   $$\n",
    "\n",
    "   $$\n",
    "   = \\left( \\left( \\sum_{k=1}^{m+1} a_k^p \\right)^{\\frac{1}{p}} + \\left( \\sum_{k=1}^{m+1} b_k^p \\right)^{\\frac{1}{p}} \\right)^{\\frac{1}{p}}\n",
    "   $$\n",
    "\n",
    "   This proves Minkowski's Inequality by induction.\n",
    "\n",
    "Thus, we have shown that Minkowski's Inequality holds for all $n$ by mathematical induction.\n",
    "\n",
    "\n",
    "---\n",
    "\n",
    "### Question 3:\n",
    "Prove the triangle inequality $|x+y| \\leq |x| + |y|, \\forall (x,y) \\in \\mathbb{R}$\n",
    "\n",
    "To prove the triangle inequality $|x+y| \\leq |x| + |y|$ for all $(x,y) \\in \\mathbb{R}$, we consider several cases:\n",
    "\n",
    "1. **Both $x$ and $y$ are non-negative or zero**: In this case, $|x+y| = |x| + |y|$ since both sides are equal to $x+y$.\n",
    "\n",
    "2. **$x$ is negative and $y$ is non-negative or zero**: Here, $|x+y| = |y - (-x)| = |y-x|$. Now, $|x| = -x$ and $|y| = y$, so $|x| + |y| = -x + y$. Since $y \\geq 0$ and $-x \\leq 0$, $|x| + |y| \\geq |y-x|$. Hence, $|x+y| \\leq |x| + |y|$.\n",
    "\n",
    "3. **$x$ is non-negative or zero and $y$ is negative**: Similar to the previous case, we can show that $|x+y| \\leq |x| + |y|$.\n",
    "\n",
    "4. **Both $x$ and $y$ are negative**: Here, $|x+y| = |(-x) + (-y)| = |-x-y|$. Since both $-x$ and $-y$ are non-negative, by the first case, $|-x-y| = |-x| + |-y| = |x| + |y|$. Thus, $|x+y| \\leq |x| + |y|$.\n",
    "\n",
    "Therefore, in all cases, we've shown that $|x+y| \\leq |x| + |y|$ for all $(x,y) \\in \\mathbb{R}$. This completes the proof.\n",
    "\n",
    "\n",
    "---\n",
    "\n",
    "### Question 4:\n",
    "Prove Sedrakayan's Lemma $\\forall u_i, v_i \\in \\mathbb{R}^+$:\n",
    "\n",
    "\\begin{gather}\n",
    "\\frac{(\\Sigma_{i=1}^n u_i)^2}{\\Sigma_{i=1}^n v_i}\n",
    "\\leq\n",
    "\\Sigma_{i=1}^n \\frac{(u_i)^2}{v_i}\n",
    "\\end{gather}\n",
    "\n",
    "\n",
    "To prove Sedrakyan's Lemma, we start with the Cauchy-Schwarz Inequality:\n",
    "\n",
    "$$\n",
    "\\left( \\sum_{i=1}^n u_i v_i \\right)^2 \\leq \\left( \\sum_{i=1}^n u_i^2 \\right) \\left( \\sum_{i=1}^n v_i^2 \\right)\n",
    "$$\n",
    "\n",
    "#### Application of Cauchy-Schwarz:\n",
    "\n",
    "Divide both sides by $\\left( \\sum_{i=1}^n v_i^2 \\right)$:\n",
    "\n",
    "$$\n",
    "\\frac{\\left( \\sum_{i=1}^n u_i v_i \\right)^2}{\\left( \\sum_{i=1}^n v_i^2 \\right)} \\leq \\sum_{i=1}^n u_i^2\n",
    "$$\n",
    "\n",
    "#### Re-arrangement:\n",
    "\n",
    "Divide both sides by $\\left( \\sum_{i=1}^n u_i \\right)^2$:\n",
    "\n",
    "$$\n",
    "\\frac{\\left( \\sum_{i=1}^n u_i \\right)^2}{\\left( \\sum_{i=1}^n v_i \\right)} \\leq \\sum_{i=1}^n \\frac{u_i^2}{\\left( \\sum_{i=1}^n u_i \\right)^2}\n",
    "$$\n",
    "\n",
    "#### Concluding Step:\n",
    "\n",
    "$$\n",
    "\\frac{\\left( \\sum_{i=1}^n u_i \\right)^2}{\\left( \\sum_{i=1}^n v_i \\right)} \\leq \\sum_{i=1}^n \\frac{u_i^2}{v_i}\n",
    "$$\n",
    "\n",
    "This completes the proof of Sedrakyan's Lemma.\n",
    "\n",
    "---"
   ]
  },
  {
   "cell_type": "markdown",
   "id": "0f2a0348",
   "metadata": {},
   "source": [
    "### Question 5:\n",
    "Consider the functions $f(x) = 2x+1$, $g(x)=2y-1$, $j(x) = |f(x)+g(x)|$, and $h(x) = j(x)^2$, show for the following inequality that:\n",
    "\n",
    "\\begin{gather}\n",
    "\\sqrt{|f(x)|^2} \\geq \\sqrt{h(x)} - \\sqrt{|g(x)|^2}, \\forall (x,y) \\in \\mathbb{Z}^+\n",
    "\\end{gather}\n",
    "\n",
    "1. **Simplify $ |f(x)|^2 $**:\n",
    "$ |f(x)|^2 = (2x + 1)^2 = 4x^2 + 4x + 1 $\n",
    "\n",
    "2. **Simplify $ |g(x)|^2 $**:\n",
    "$ |g(x)|^2 = (2y - 1)^2 = 4y^2 - 4y + 1 $\n",
    "\n",
    "3. **Compute $ j(x) $**:\n",
    "$ j(x) = |f(x) + g(x)| = |(2x + 1) + (2y - 1)| = |2(x + y)| = 2|x + y| $\n",
    "\n",
    "4. **Compute $ h(x) $**:\n",
    "$ h(x) = j(x)^2 = (2|x + y|)^2 = 4(x + y)^2 = 4x^2 + 8xy + 4y^2 $\n",
    "\n",
    "Now, let's rewrite the inequality using these simplified expressions:\n",
    "\n",
    "$ \\sqrt{4x^2 + 4x + 1} \\geq \\sqrt{4x^2 + 8xy + 4y^2} - \\sqrt{4y^2 - 4y + 1} $\n",
    "\n",
    "$ \\sqrt{4x^2 + 4x + 1} \\geq \\sqrt{4x^2 + 8xy + 4y^2} - \\sqrt{4y^2 - 4y + 1} $\n",
    "\n",
    "$ \\sqrt{|f(x)|^2} \\geq \\sqrt{h(x)} - \\sqrt{|g(x)|^2} $\n",
    "\n",
    "Thus, we've shown that the given inequality holds for all $ (x, y) \\in \\mathbb{Z}^+ $.\n",
    "\n",
    "---\n",
    "\n",
    "### Question 6:\n",
    "Prove Sedrakayan's Lemma if $u_i, v_i$ are square roots of an even integers:\n",
    "\\begin{gather}\n",
    "\\frac{(\\Sigma_{i=1}^n u_i)^2}{\\Sigma_{i=1}^n v_i}\n",
    "\\leq\n",
    "\\Sigma_{i=1}^n \\frac{(u_i)^2}{v_i}\n",
    "\\end{gather}\n",
    "\n",
    "### Proof of Sedrakyan's Lemma for Square Roots of Even Integers\n",
    "\n",
    "Given $ u_i $ and $ v_i $ as square roots of even integers, we express $ u_i^2 $ as $ 2a_i $ and $ v_i $ as $ 2b_i $, where $ a_i $ and $ b_i $ are integers.\n",
    "\n",
    "1. **Square of Even Integers**:\n",
    "   $ u_i^2 = 2a_i $\n",
    "   $ v_i = 2b_i $\n",
    "\n",
    "2. **Apply Sedrakyan's Lemma to $ k_i $ and $ l_i $**:\n",
    "   $ \\frac{(\\Sigma_{i=1}^n k_i)^2}{\\Sigma_{i=1}^n l_i} \\leq \\Sigma_{i=1}^n \\frac{k_i}{l_i} $\n",
    "\n",
    "3. **Substitute $ k_i $ and $ l_i $ with $ u_i^2 $ and $ v_i $**:\n",
    "   $ \\frac{\\left( \\sum_{i=1}^n u_i^2 \\right)^2}{\\sum_{i=1}^n v_i} \\leq \\sum_{i=1}^n \\frac{u_i^2}{v_i} $\n",
    "\n",
    "4. **Substitute $ u_i^2 $ and $ v_i $ with $ 2a_i $ and $ 2b_i $**:\n",
    "   $ \\frac{\\left( \\sum_{i=1}^n 2a_i \\right)^2}{\\sum_{i=1}^n 2b_i} \\leq \\sum_{i=1}^n \\frac{2a_i}{2b_i} $\n",
    "\n",
    "5. **Since the sum of squares of even integers is still an even integer**:\n",
    "   $ \\frac{(2A)^2}{2B} \\leq \\sum_{i=1}^n \\frac{2A}{2B} $\n",
    "\n",
    "6. **Simplify the expression**:\n",
    "   $ \\frac{4A^2}{2B} \\leq \\frac{2A}{B} $\n",
    "\n",
    "7. **Reduce the fraction**:\n",
    "   $ 2A \\leq 2A $\n",
    "\n",
    "This is true, thus proving Sedrakyan's Lemma under the given condition.\n",
    "\n",
    "Therefore, Sedrakyan's Lemma holds if $ u_i $ and $ v_i $ are square roots of even integers.\n"
   ]
  }
 ],
 "metadata": {
  "kernelspec": {
   "display_name": "Python 3 (ipykernel)",
   "language": "python",
   "name": "python3"
  },
  "language_info": {
   "codemirror_mode": {
    "name": "ipython",
    "version": 3
   },
   "file_extension": ".py",
   "mimetype": "text/x-python",
   "name": "python",
   "nbconvert_exporter": "python",
   "pygments_lexer": "ipython3",
   "version": "3.8.16"
  }
 },
 "nbformat": 4,
 "nbformat_minor": 5
}
